Simplify `pure_beta_equivTheory`
Plus some minor tidying

meta-theory/pure_beta_equivScript.sml
@@ -1,8 +1,8 @@
 (*
   Theorem beta_equivalence:
-    App (Lam x body) arg ≅ CA_subst x arg body
+    App (Lam x body) arg ≅ ca_subst x arg body
 
-  where CA_subst is the capture-avoiding substitution of the free variables "x"
+  where ca_subst is the capture-avoiding substitution of the free variables "x"
   in the expression "body" with the expression "arg"
 
   The main theorem above states that two beta-equivalent expressions
@@ -23,9 +23,7 @@ val _ = new_theory "pure_beta_equiv";
 
 
 Definition fresh_var_def:
-  fresh_var v xs = if ¬MEM v xs
-                   then v
-                   else fresh_var (v ++ "'") xs
+  fresh_var v xs = if ¬MEM v xs then v else fresh_var (v ++ "'") xs
 Termination
   WF_REL_TAC ‘measure (λ(v,xs). (LENGTH (FLAT xs) + 1) - LENGTH v)’ \\ rw[]
   \\ Induct_on ‘xs’ \\ fs[] \\ rpt strip_tac \\ fs[]
@@ -39,10 +37,28 @@ Proof
   \\ IF_CASES_TAC \\ fs[]
 QED
 
+Theorem fresh_var_avoid_eq:
+  ∀x avoid1 avoid2.
+    set avoid1 = set avoid2
+  ⇒ fresh_var x avoid1 = fresh_var x avoid2
+Proof
+  recInduct fresh_var_ind >> rw[EXTENSION] >>
+  once_rewrite_tac[fresh_var_def] >> gvs[] >>
+  IF_CASES_TAC >> gvs[]
+QED
+
+Theorem fresh_var_DISJ:
+  ∀v l. (fresh_var v l = v ∧ ¬ MEM v l) ∨ (fresh_var v l ≠ v ∧ MEM v l)
+Proof
+  once_rewrite_tac[fresh_var_def] >> rw[] >>
+  metis_tac[fresh_var_correctness]
+QED
+
 Definition fresh_var_list_def:
   fresh_var_list []      to_avoid = [] ∧
-  fresh_var_list (x::xs) to_avoid = let fresh = fresh_var x to_avoid;
-                                    in ((x,fresh)::fresh_var_list xs (fresh::to_avoid))
+  fresh_var_list (x::xs) to_avoid =
+    let fresh = fresh_var x to_avoid in
+    ((x,fresh)::fresh_var_list xs (fresh::to_avoid))
 End
 
 Theorem MAP_FST_fresh_var_list:
@@ -73,100 +89,67 @@ Proof
   \\ fs[]
 QED
 
-Theorem perm_exp_size_lemma:
- ∀ e. list_size char_size s = list_size char_size s'
-      ⇒ exp_size (perm_exp s s' e) = exp_size e
+Theorem fresh_var_list_SUBSET:
+  ∀l avoid.
+    set l ⊆ set (MAP SND (fresh_var_list l avoid)) ∪ set avoid
 Proof
-  GEN_TAC
-  \\ completeInduct_on ‘exp_size e’
-  \\ fs[PULL_FORALL]
-  \\ rw[]
-  \\ Cases_on ‘e’
-  THEN1(
-   fs[perm_exp_def, perm1_def]
-   \\ fs[exp_size_def]
-   \\ IF_CASES_TAC \\ fs[]
-   \\ IF_CASES_TAC \\ fs[]
-  )
-  THEN1(
-   fs[perm_exp_def, perm1_def]
-   \\ fs[exp_size_def]
-   \\ Induct_on ‘l’ \\ fs[]
-   \\ rw[] \\ fs[exp_size_def]
-  )
-  THEN1(
-   fs[perm_exp_def, perm1_def]
-   \\ fs[exp_size_def]
-  )
-  THEN1(
-   fs[perm_exp_def, perm1_def]
-   \\ fs[exp_size_def]
-   \\ IF_CASES_TAC \\ fs[]
-   \\ IF_CASES_TAC \\ fs[]
-  )
-  THEN1(
-   fs[perm_exp_def,exp_size_def]
-   \\ Induct_on ‘l’ \\ fs[]
-   \\ strip_tac
-   \\ fs[exp_size_def]
-   \\ rw[] \\ fs[exp_size_def]
-   \\ Cases_on ‘h’ \\ fs[] \\ fs[exp_size_def] \\ rw[]
-   \\ fs[perm_exp_def,exp_size_def,perm1_def]
-   \\ IF_CASES_TAC \\ fs[perm_exp_def,exp_size_def]
-   \\ IF_CASES_TAC \\ fs[perm_exp_def,exp_size_def]
-  )
+  Induct >> rw[fresh_var_list_def]
+  >- (simp[Once fresh_var_def] >> IF_CASES_TAC >> gvs[]) >>
+  gvs[SUBSET_DEF] >> rw[] >>
+  last_x_assum drule >>
+  disch_then (qspec_then `fresh_var h avoid::avoid` assume_tac) >> gvs[]
 QED
 
-Definition exp_size'_def:
-  exp_size' (Var        a) = 1                                   ∧
-  exp_size' (Prim   a0 a1) = 1 + (op_size a0 + exp3_size' a1)    ∧
-  exp_size' (App    a0 a1) = 1 + (exp_size' a0 + exp_size' a1)   ∧
-  exp_size' (Lam    a0 a1) = 1 + (1 + exp_size' a1)              ∧
-  exp_size' (Letrec a0 a1) = 1 + (exp1_size' a0 + exp_size' a1)  ∧
-  exp1_size' [] = 0                                              ∧
-  exp1_size' (a0::a1) = 1 + (exp2_size' a0 + exp1_size' a1)      ∧
-  exp2_size' (a0, a1) = 1 + (1 + exp_size' a1)                   ∧
-  exp3_size' [] = 0                                              ∧
-  exp3_size' (a0::a1) = 1 + (exp_size' a0 + exp3_size' a1)
+Theorem fresh_var_list_avoid_eq:
+  ∀l avoid1 avoid2.
+    set avoid1 = set avoid2
+  ⇒ fresh_var_list l avoid1 = fresh_var_list l avoid2
+Proof
+  Induct >> rw[fresh_var_list_def]
+  >- (
+    once_rewrite_tac[fresh_var_def] >>
+    drule fresh_var_avoid_eq >> gvs[EXTENSION]
+    ) >>
+  first_x_assum irule >> gvs[] >>
+  drule fresh_var_avoid_eq >> simp[]
+QED
+
+Definition exp_size_alt_def:
+  exp_size_alt (Var v) = 1 ∧
+  exp_size_alt (Prim op xs) = 1 + SUM (MAP exp_size_alt xs) ∧
+  exp_size_alt (App e1 e2) = 1 + exp_size_alt e1 + exp_size_alt e2 ∧
+  exp_size_alt (Lam x e) = 1 + exp_size_alt e ∧
+  exp_size_alt (Letrec fns e) =
+    1 + exp_size_alt e + SUM (MAP (λ(v,fn). exp_size_alt fn) fns)
+Termination
+  WF_REL_TAC `measure (λe. exp_size e)` >> rw[exp_size_def]
+  >- (Induct_on `fns` >> rw[] >> gvs[exp_size_def])
+  >- (Induct_on `xs` >> rw[] >> gvs[exp_size_def])
 End
 
-Theorem exp_size'_lemma:
-  ∀ r. MEM (q,r) l' ⇒ exp_size' r < exp1_size' l'
+Theorem perm_exp_size:
+  ∀e x y. exp_size_alt e = exp_size_alt (perm_exp x y e)
 Proof
-  Induct_on ‘l'’ \\ fs[] \\ Cases \\ rw[] \\ fs[exp_size'_def]
-  \\ res_tac \\ fs[]
-QED
-
-Theorem perm_exp_size'_mono:
-  ∀ s s' e. exp_size' (perm_exp s s' e) = exp_size' e
-Proof
-  rw[]
-  \\ completeInduct_on ‘exp_size' e’
-  \\ rw[]
-  \\ fs[PULL_FORALL]
-  \\ Cases_on ‘e’
-  \\ fs[exp_size'_def,perm_exp_def,perm1_def]
-  THEN1 (
-    Induct_on ‘l’ \\ fs[]
-    \\ fs[exp_size'_def,perm_exp_def,perm1_def]
-  )
-  THEN1 (
-    Induct_on ‘l’ \\ fs[]
-    \\ Cases
-    \\ fs[exp_size'_def,perm_exp_def,perm1_def]
-  )
+  recInduct exp_size_alt_ind >> rw[exp_size_alt_def, perm_exp_def]
+  >- (AP_TERM_TAC >> rw[MAP_MAP_o, combinTheory.o_DEF, MAP_EQ_f])
+  >- metis_tac[]
+  >- (
+    pop_assum (once_rewrite_tac o single) >> simp[] >>
+    AP_TERM_TAC >> rw[MAP_MAP_o, combinTheory.o_DEF, MAP_EQ_f] >>
+    pairarg_tac >> gvs[] >> res_tac >> simp[]
+    )
 QED
 
 Definition perm_exp_list_def:
   perm_exp_list [] e = e ∧
-  perm_exp_list ((old,new)::binds) e = perm_exp_list binds (perm_exp old new e)
+  perm_exp_list ((old,new)::binds) e = perm_exp old new (perm_exp_list binds e)
 End
 
-Theorem perm_exp_list_size'_mono:
-  ∀ binds e. exp_size' (perm_exp_list binds e) = exp_size' e
+Theorem perm_exp_list_size:
+  ∀ binds e. exp_size_alt (perm_exp_list binds e) = exp_size_alt e
 Proof
-  recInduct perm_exp_list_ind
-  \\ rw[] \\ fs[perm_exp_list_def,perm_exp_size'_mono]
+  recInduct perm_exp_list_ind >> rw[perm_exp_list_def] >>
+  metis_tac[perm_exp_size]
 QED
 
 Theorem exp_alpha_perm_exp_list:
@@ -175,857 +158,465 @@ Theorem exp_alpha_perm_exp_list:
     ∧ (DISJOINT (set (MAP SND binds)) (freevars e))
     ⇒ exp_alpha e (perm_exp_list binds e)
 Proof
-  recInduct perm_exp_list_ind
-  \\ conj_tac
-  THEN1 (
-    rw[]
-    \\ fs[perm_exp_list_def]
-    \\ fs[exp_alpha_refl]
-  )
-  \\ rw[]
-  \\ fs[perm_exp_list_def]
-  \\ irule exp_alpha_Trans
-  \\ qexists_tac  ‘(perm_exp old new e)’
-  \\ conj_tac
-  THEN1 (irule exp_alpha_perm_irrel \\ fs[])
-  \\ last_assum irule
-  \\ fs[freevars_perm_exp]
-  \\ fs[EXTENSION,DISJOINT_DEF] \\  metis_tac[]
+  recInduct perm_exp_list_ind >> rw[perm_exp_list_def, exp_alpha_refl] >>
+  irule exp_alpha_Trans >> qexists_tac `perm_exp old new e` >>
+  irule_at Any exp_alpha_perm_irrel >> simp[] >>
+  irule exp_alpha_perm_closed >>
+  last_x_assum irule >> simp[]
 QED
 
-Theorem exp_alpha_perm_exp_list_trans:
-  ∀ binds e e'.
-      (DISJOINT (set (MAP FST binds)) (freevars e'))
-    ∧ (DISJOINT (set (MAP SND binds)) (freevars e'))
-    ∧ exp_alpha e e'
-    ⇒ exp_alpha e (perm_exp_list binds e')
+Theorem freevars_perm_exp_list_unchanged:
+  ∀ binds e.
+    DISJOINT (set (MAP FST binds)) (freevars e) ∧
+    DISJOINT (set (MAP SND binds)) (freevars e)
+  ⇒ freevars (perm_exp_list binds e) = freevars e
 Proof
-  recInduct perm_exp_list_ind
-  \\ conj_tac
-  THEN1 (fs[perm_exp_list_def])
-  \\ rw[]
-  \\ fs[perm_exp_list_def]
-  \\ irule exp_alpha_Trans
-  \\ qexists_tac ‘(perm_exp old new e')’
-  \\ conj_tac
-  THEN1 (
-    irule exp_alpha_Trans
-    \\ qexists_tac ‘e'’
-    \\ fs[]
-    \\ irule exp_alpha_perm_irrel \\ fs[]
-  )
-  \\ irule exp_alpha_perm_exp_list \\ fs[]
-  \\ fs[freevars_perm_exp]
-  \\ fs[EXTENSION,DISJOINT_DEF] \\  metis_tac[]
+  recInduct perm_exp_list_ind >> rw[perm_exp_list_def] >>
+  gvs[freevars_eqvt] >>
+  rw[EXTENSION, perm1_def] >>
+  eq_tac >> rw[]
+  >- (EVERY_CASE_TAC >> gvs[])
+  >- (qexists_tac `x` >> EVERY_CASE_TAC >> gvs[])
 QED
 
-Triviality FILTER_MEM_INTERSECTION:
-  ∀ l1 l2. set (FILTER (λx. MEM x l2) l1) = set l1 ∩ set l2
-Proof
-  Induct \\ fs[]
-  \\ rw[]
-  \\ fs[EXTENSION,INTER_DEF] \\ metis_tac[]
-QED
-
-Triviality DISJOINT_UNION_DIFF:
-   DISJOINT A (B DIFF D)
- ∧ DISJOINT A (C DIFF D) ⇒ DISJOINT A (B ∪ C DIFF D)
-Proof
- fs[EXTENSION,DISJOINT_DEF] \\ metis_tac[]
-QED
-
-Triviality DIFF_SUBSET_UNION:
-  A DIFF B ⊆ C ⇒ A ⊆ C ∪ B
-Proof
-  fs[EXTENSION,DISJOINT_DEF,SUBSET_DEF] \\ metis_tac[]
-QED
-
-Triviality UNION_SYM:
-  ∀ A B. A ∪ B = B ∪ A
-Proof
-  fs[EXTENSION,UNION_DEF] \\ metis_tac[]
-QED
-
-Definition avoid_vars_def:
-  avoid_vars avoid (Var x) = (Var x) ∧
-  avoid_vars avoid (Prim op es) = Prim op (MAP (avoid_vars avoid) es) ∧
-  avoid_vars avoid (Lam x e) = (
-                 let fresh = fresh_var x avoid           in
-                 let e'    = avoid_vars (fresh::x::avoid) e
-                 in Lam fresh (perm_exp x fresh e'))                  ∧
-  avoid_vars avoid (App e1 e2) = App (avoid_vars avoid e1)
-                                     (avoid_vars avoid e2)            ∧
-  avoid_vars avoid (Letrec lcs e) =
-     let clashes     = nub (FILTER (λx. MEM x avoid) (MAP FST lcs))  in
-     let freshes     = fresh_var_list clashes (MAP FST lcs ++ avoid) in
-     let new_avoids  = MAP FST lcs ++ avoid ++ MAP SND freshes       in
-     let lcs_bodies' = MAP (\x. avoid_vars new_avoids (SND x)) lcs   in
-     let lcs'        = ZIP (MAP FST lcs,lcs_bodies')                 in
-     let body'       = avoid_vars new_avoids e
-     in  perm_exp_list freshes (Letrec lcs' body')
+Definition freshen_def:
+  freshen avoid (Var x) = (Var x) ∧
+  freshen avoid (Prim op es) = Prim op (MAP (freshen avoid) es) ∧
+  freshen avoid (Lam x e) =
+    (let y = fresh_var x avoid in
+    Lam y (freshen (y::avoid) (perm_exp x y e))) ∧
+  freshen avoid (App e1 e2) = App (freshen avoid e1) (freshen avoid e2) ∧
+  freshen avoid (Letrec lcs e) =
+    let fresh_vars = fresh_var_list (MAP FST lcs) avoid in
+    let fresh_lcs = MAP (λ(n,e). (n, freshen (MAP SND fresh_vars ++ avoid) e)) lcs in
+    let fresh_e = freshen (MAP SND fresh_vars ++ avoid) e in
+    perm_exp_list fresh_vars (Letrec fresh_lcs fresh_e)
 Termination
-  WF_REL_TAC ‘measure (exp_size' o SND)’ \\ fs[exp_size'_def]
-  \\ reverse (rpt conj_tac)
-  THEN1 (
-    rw[]
-    \\ Induct_on ‘es’ \\ fs[]
-    \\ rw[] \\ fs[exp_size'_def]
-  )
-  \\ rw[]
-  \\ imp_res_tac exp_size'_lemma \\ fs[]
+  WF_REL_TAC `measure (λ(_,e). exp_size_alt e)` >> rw[exp_size_alt_def] >>
+  simp[GSYM perm_exp_size, perm_exp_list_size]
+  >- (Induct_on `lcs` >> rw[] >> gvs[])
+  >- (Induct_on `es` >> rw[] >> gvs[] >> DECIDE_TAC)
 End
 
-Theorem exp_alpha_avoid_vars:
-  ∀ avoid e. freevars e ⊆ (set avoid) ⇒ exp_alpha e (avoid_vars avoid e)
+Theorem exp_alpha_freshen:
+  ∀ avoid e. freevars e ⊆ (set avoid) ⇒ exp_alpha e (freshen avoid e)
 Proof
-  recInduct avoid_vars_ind
-  \\ rw[]
-  THEN1 (
-    fs[avoid_vars_def]
-    \\ fs[exp_alpha_refl]
-  )
-  THEN1 (
-    fs[avoid_vars_def]
-    \\ irule exp_alpha_Prim
-    \\ fs[EVERY2_EVERY]
-    \\ fs[ZIP_MAP]
-    \\ fs[EVERY_MEM]
-    \\ Cases
-    \\ fs[MAP_MAP_o,combinTheory.o_DEF]
-    \\ fs[MEM_MAP] \\ rw[]
-    \\ res_tac \\ fs[]
-    \\ pop_assum irule
-    \\ irule SUBSET_TRANS
-    \\ qexists_tac ‘BIGUNION (set (MAP (λe. freevars e) es))’
-    \\ fs[]
-    \\ fs[EXTENSION,BIGUNION,SUBSET_DEF] \\ rw[]
-    \\ qexists_tac ‘freevars q’ \\ fs[]
-    \\ fs[MEM_MAP]
-    \\ qexists_tac ‘q’ \\ fs[]
-  )
-  THEN1 (
-    fs[avoid_vars_def]
-    \\ Cases_on ‘fresh_var x avoid = x’ \\ fs[perm_exp_id] \\ rw[]
-    THEN1 (
-      fs[DELETE_SUBSET_INSERT]
-      \\ irule exp_alpha_Lam \\ fs[]
+  recInduct freshen_ind >> rw[freshen_def, exp_alpha_refl]
+  >- (
+    irule exp_alpha_Prim >> rw[LIST_REL_EL_EQN, EL_MAP] >>
+    last_x_assum irule >> simp[EL_MEM] >>
+    gvs[SUBSET_DEF, PULL_EXISTS, MEM_MAP] >> rw[] >>
+    first_x_assum irule >> goal_assum (drule_at Any) >> simp[EL_MEM]
     )
-    \\ fs[DELETE_SUBSET_INSERT]
-    \\ last_x_assum mp_tac
-    \\ impl_tac THEN1 (fs[EXTENSION,SUBSET_DEF] \\ metis_tac[])
-    \\ disch_tac
-    \\ irule exp_alpha_Trans
-    \\ qexists_tac ‘Lam (fresh_var x avoid) (perm_exp x (fresh_var x avoid) e)’
-    \\ conj_tac
-    THEN1 (
-      irule exp_alpha_Alpha
-      \\ qspecl_then [‘x’,‘avoid’] assume_tac fresh_var_correctness
-      \\ fs[EXTENSION,SUBSET_DEF] \\ metis_tac[]
+  >- (
+    Cases_on `fresh_var x avoid = x` >> gvs[perm_exp_id]
+    >- (
+      irule exp_alpha_Lam >> first_x_assum irule >>
+      gvs[SUBSET_INSERT_DELETE]
+      ) >>
+    `¬ MEM (fresh_var x avoid) avoid` by simp[fresh_var_correctness] >>
+    qabbrev_tac `y = fresh_var x avoid` >>
+    irule exp_alpha_Trans >>
+    qexists_tac `Lam y (perm_exp x y e)`  >>
+    irule_at Any exp_alpha_Lam >>
+    first_x_assum (irule_at Any) >>
+    gvs[freevars_eqvt, SUBSET_DEF, perm1_def] >>
+    conj_tac >- metis_tac[] >>
+    irule exp_alpha_Alpha >> simp[] >>
+    metis_tac[]
     )
-    \\ irule exp_alpha_Lam
-    \\ irule exp_alpha_perm_closed
-    \\ last_x_assum irule
-    \\ fs[EXTENSION,SUBSET_DEF] \\ metis_tac[]
-  )
-  THEN1 (
-    fs[avoid_vars_def]
-    \\ irule exp_alpha_App \\ fs[]
-  )
-  \\ fs[avoid_vars_def]
-  \\ ‘freevars e ⊆ set (MAP FST lcs) ∪ set avoid
-      ∪ set (MAP SND
-             (fresh_var_list (nub (FILTER (λx. MEM x avoid) (MAP FST lcs)))
-               (MAP FST lcs ++ avoid)))’ by (
-     fs[EXTENSION,SUBSET_DEF] \\ metis_tac[]
-  )
-  \\ res_tac \\ fs[] \\ rw[]
-  \\ irule exp_alpha_perm_exp_list_trans
-  \\ conj_tac
-  THEN1 (
-    fs[ZIP_MAP]
-    \\ fs[MAP_MAP_o,combinTheory.o_DEF]
-    \\ fs[freevars_perm_exp]
-    \\ fs[MAP_FST_fresh_var_list]
-    \\ fs[MAP_MAP_o,combinTheory.o_DEF]
-    \\ fs[FILTER_MEM_INTERSECTION]
-    \\ fs[EXTENSION,DISJOINT_DEF,freevars_perm_exp] \\ metis_tac[]
-  )
-  \\ conj_tac
-  THEN1 (
-    fs [ZIP_MAP]
-    \\ fs[MAP_MAP_o,combinTheory.o_DEF]
-    \\ drule (GSYM exp_alpha_freevars)
-    \\ disch_tac \\ fs[]
-    \\ irule DISJOINT_UNION_DIFF
-    \\ conj_tac
-    THEN1 (
-      irule DISJOINT_SUBSET
-      \\ qexists_tac ‘set (MAP FST lcs ++ avoid)’
-      \\ conj_tac THEN1 (fs[fresh_var_list_correctness])
-      \\ fs[EXTENSION,SUBSET_DEF] \\ metis_tac[]
+  >- (irule exp_alpha_App >> res_tac >> simp[])
+  >- (
+    gvs[DIFF_SUBSET] >>
+    qpat_x_assum `_ ⇒ exp_alpha _ _` mp_tac >>
+    impl_keep_tac
+    >- (
+      qspecl_then [`MAP FST lcs`,`avoid`] assume_tac fresh_var_list_SUBSET >>
+      gvs[SUBSET_DEF] >> rw[] >> metis_tac[]
+      ) >>
+    strip_tac >>
+    imp_res_tac exp_alpha_freevars >> pop_assum (assume_tac o GSYM) >>
+    `∀p1 p2. MEM (p1,p2) lcs ⇒
+      exp_alpha p2
+      (freshen (MAP SND (fresh_var_list (MAP FST lcs) avoid) ++ avoid) p2)` by (
+      rw[] >> first_x_assum irule >> simp[PULL_EXISTS] >> goal_assum drule >>
+      qspecl_then [`MAP FST lcs`,`avoid`] assume_tac fresh_var_list_SUBSET >>
+      gvs[SUBSET_DEF] >> rw[] >>
+      qsuff_tac `MEM x (MAP FST lcs) ∨ MEM x avoid` >- metis_tac[] >>
+      last_x_assum irule >> simp[MEM_MAP, PULL_EXISTS, EXISTS_PROD] >>
+      goal_assum drule >> goal_assum drule) >>
+    last_x_assum kall_tac >>
+    qmatch_goalsub_abbrev_tac `exp_alpha _ (perm_exp_list l exp)` >>
+    irule exp_alpha_Trans >> qexists_tac `exp` >> rw[]
+    >- (
+      unabbrev_all_tac >> irule exp_alpha_Letrec >>
+      simp[MAP_MAP_o, combinTheory.o_DEF, LAMBDA_PROD] >> simp[GSYM FST_THM] >>
+      rw[LIST_REL_EL_EQN, EL_MAP, UNCURRY] >>
+      first_x_assum irule >>
+      qexists_tac `FST (EL n lcs)` >> gvs[EL_MEM]
+      ) >>
+    irule exp_alpha_perm_exp_list >> unabbrev_all_tac >>
+    simp[MAP_FST_fresh_var_list] >>
+    simp[MAP_MAP_o, combinTheory.o_DEF, LAMBDA_PROD] >>
+    simp[GSYM FST_THM, DISJOINT_DIFF] >>
+    `MAP (λ(p1,p2).
+      freevars (freshen
+        (MAP SND (fresh_var_list (MAP FST lcs) avoid) ++ avoid) p2)) lcs =
+      MAP (λ(p1,p2). freevars p2) lcs` by (
+        rw[MAP_EQ_f] >> pairarg_tac >> gvs[] >>
+        first_x_assum drule >> strip_tac >>
+        imp_res_tac exp_alpha_freevars >> simp[]) >>
+    gvs[] >> pop_assum kall_tac >>
+    qspecl_then [`MAP FST lcs`,`avoid`]
+      assume_tac fresh_var_list_correctness >>
+    gvs[DISJOINT_DEF, EXTENSION] >> rw[] >>
+    pop_assum (qspec_then `x` assume_tac) >> gvs[] >>
+    Cases_on `MEM x (MAP FST lcs)` >> gvs[] >>
+    gvs[SUBSET_DEF] >>
+    last_x_assum (qspec_then `x` assume_tac) >>
+    last_x_assum (qspec_then `x` assume_tac) >> gvs[]
     )
-    \\ irule DISJOINT_SUBSET
-    \\ qexists_tac
-       ‘freevars e
-       ∪ BIGUNION (set (MAP
-           (λx.freevars (avoid_vars (MAP FST lcs
-                                     ++ avoid
-                                     ++  MAP SND
-                                          (fresh_var_list
-                                           (nub (FILTER (λx. MEM x avoid) (MAP FST lcs)))
-                                           (MAP FST lcs ++ avoid))) (SND x)))
-           lcs))’
-    \\ reverse conj_tac THEN1 (fs[EXTENSION,SUBSET_DEF] \\ metis_tac[])
-    \\ fs[DISJOINT_BIGUNION]
-    \\ conj_tac
-    THEN1 (
-      once_rewrite_tac[DISJOINT_SYM]
-      \\ irule DISJOINT_SUBSET
-      \\ qexists_tac ‘set (MAP FST lcs ++ avoid)’
-      \\ conj_tac THEN1 (fs[fresh_var_list_correctness])
-      \\ fs[EXTENSION,SUBSET_DEF] \\ metis_tac[]
-    )
-    \\ fs[MEM_MAP] \\ rw[]
-    \\ last_x_assum (qspec_then ‘x’ assume_tac)
-    \\ Cases_on ‘x’ \\ fs[]
-    \\ pop_assum mp_tac
-    \\ impl_tac \\ fs[]
-    \\ impl_tac
-    THEN1 (
-      irule SUBSET_TRANS
-      \\ qexists_tac ‘BIGUNION (set (MAP (λ(fn,e). freevars e) lcs))’
-      \\ reverse conj_tac THEN1 (fs[EXTENSION,SUBSET_DEF] \\ metis_tac[])
-      \\ irule SUBSET_BIGUNION_I
-      \\ fs[MEM_MAP]
-      \\ qexists_tac ‘(q,r)’ \\ fs[]
-    )
-    \\ disch_tac
-    \\ drule (GSYM exp_alpha_freevars)
-    \\ disch_tac \\ fs[]
-    \\ once_rewrite_tac[DISJOINT_SYM]
-    \\ irule DISJOINT_SUBSET
-    \\ qexists_tac ‘set (MAP FST lcs ++ avoid)’
-    \\ conj_tac THEN1 (fs[fresh_var_list_correctness])
-    \\ fs[]
-    \\ once_rewrite_tac[UNION_SYM]
-    \\ irule DIFF_SUBSET_UNION
-    \\ irule SUBSET_TRANS
-    \\ qexists_tac ‘BIGUNION (set (MAP (λ(fn,e). freevars e) lcs)) DIFF
-                    set (MAP FST lcs)’
-    \\ reverse conj_tac THEN1 (fs[EXTENSION,SUBSET_DEF] \\ metis_tac[])
-    \\ qsuff_tac ‘freevars r ⊆ BIGUNION (set (MAP (λ(fn,e). freevars e) lcs))’
-    THEN1 (fs[EXTENSION,SUBSET_DEF] \\ metis_tac[])
-    \\ irule SUBSET_BIGUNION_I
-    \\ fs[MEM_MAP]
-    \\ qexists_tac ‘(q,r)’ \\ fs[]
-  )
-  \\ fs[ZIP_MAP]
-  \\ fs[MAP_MAP_o,combinTheory.o_DEF]
-  \\ irule exp_alpha_Letrec
-  \\ rw[]
-  THEN1 (fs[MAP_MAP_o,combinTheory.o_DEF,MAP_EQ_f])
-  \\ fs[MAP_MAP_o,combinTheory.o_DEF,MAP_EQ_f]
-  \\ fs[EVERY2_EVERY]
-  \\ fs[ZIP_MAP]
-  \\ fs[MAP_MAP_o,combinTheory.o_DEF,MAP_EQ_f]
-  \\ fs[EVERY_MEM]
-  \\ Cases
-  \\ fs[MEM_MAP]
-  \\ rw[]
-  \\ Cases_on ‘x’ \\ fs[]
-  \\ res_tac \\ fs[]
-  \\ pop_assum irule
-  \\ irule SUBSET_TRANS
-  \\ qexists_tac ‘BIGUNION (set (MAP (λ(fn,e). freevars e) lcs))’
-  \\ reverse conj_tac THEN1 (fs[EXTENSION,SUBSET_DEF] \\ metis_tac[])
-  \\ irule SUBSET_BIGUNION_I
-  \\ fs[MEM_MAP]
-  \\ qexists_tac ‘(q,r)’ \\ fs[]
 QED
 
-
-
-
-(********Capture avoiding substitution**********)
-
-
-
-Definition CA_subst_def:
-   CA_subst x arg body =
-       subst x arg (avoid_vars (freevars arg ++ freevars body) body)
-End
-
-Theorem App_Lam_bisim:
-  closed (Lam x body) ∧ closed arg ⇒
-  App (Lam x body) arg ≃ subst x arg body
-Proof
-  rw [] \\ match_mp_tac eval_IMP_app_bisimilarity
-  \\ fs [eval_Let,bind_single_def]
-  \\ match_mp_tac IMP_closed_subst
-  \\ fs [] \\ fs [closed_def,FILTER_EQ_NIL,EVERY_MEM,SUBSET_DEF]
-QED
-
-Triviality app_bisimilarity_trans:
-  ∀x y z. x ≃ y ∧ y ≃ z ⇒ x ≃ z
-Proof
-  rw[]
-  \\ assume_tac transitive_app_bisimilarity
-  \\ fs[transitive_def]
-  \\ res_tac \\ fs[]
-QED
-
-Triviality app_bisimilarity_sym:
-  ∀x y. x ≃ y ⇒ y ≃ x
-Proof
-  rw[]
-  \\ assume_tac symmetric_app_bisimilarity
-  \\ fs[symmetric_def]
-QED
-
-Theorem freevars_avoid_vars_mono:
+Theorem freevars_freshen_mono:
   ∀ avoid e . freevars e ⊆ set avoid
-  ⇒ freevars (avoid_vars avoid e) = freevars e
+  ⇒ freevars (freshen avoid e) = freevars e
 Proof
   rw[]
-  \\ drule exp_alpha_avoid_vars
+  \\ drule exp_alpha_freshen
   \\ disch_tac
   \\ imp_res_tac exp_alpha_freevars
   \\ fs[]
 QED
 
+(********Capture avoiding substitution**********)
+
+Theorem App_Lam_bisim:
+  closed (Lam x body) ∧ closed arg ⇒
+  App (Lam x body) arg ≃ subst1 x arg body
+Proof
+  rw [] \\ match_mp_tac eval_IMP_app_bisimilarity
+  \\ fs [eval_Let,bind1_def]
+  \\ match_mp_tac IMP_closed_subst
+  \\ fs [] \\ fs [closed_def,FILTER_EQ_NIL,EVERY_MEM,SUBSET_DEF]
+QED
+
+Triviality app_bisimilarity_trans =
+  transitive_app_bisimilarity |> SIMP_RULE std_ss [transitive_def];
+
+Triviality app_bisimilarity_sym =
+  symmetric_app_bisimilarity |> SIMP_RULE std_ss [symmetric_def];
+
+Definition perm1_list_def:
+  perm1_list [] z = z ∧
+  perm1_list ((x,y)::rest) z = perm1 x y (perm1_list rest z)
+End
+
 Theorem boundvars_perm_exp_list:
-  ∀ binds e.
-     ALL_DISTINCT (MAP FST binds)
-  ∧  ALL_DISTINCT (MAP SND binds)
-  ∧  DISJOINT (set (MAP SND binds)) (boundvars e)
-  ⇒  boundvars (perm_exp_list binds e) ⊆
-     boundvars e DIFF (set (MAP FST binds)) ∪ set (MAP SND binds)
+  ∀l e. boundvars (perm_exp_list l e) = IMAGE (perm1_list l) (boundvars e)
 Proof
-  recInduct perm_exp_list_ind
-  \\ conj_tac THEN1 (fs[perm_exp_list_def])
-  \\ rw[]
-  \\ fs[perm_exp_list_def]
-  \\ fs[boundvars_perm_exp]
-  \\ last_x_assum mp_tac
-  \\ reverse impl_tac
-  \\ rw[]
-  \\ fs[EXTENSION,SUBSET_DEF,DISJOINT_DEF] \\ metis_tac[MEM]
+  recInduct perm_exp_list_ind >> rw[perm_exp_list_def]
+  >- (rw[EXTENSION, perm1_list_def]) >>
+  gvs[EXTENSION, boundvars_eqvt, PULL_EXISTS] >>
+  rw[perm1_list_def]
 QED
 
-Triviality DISJOINT_UNION_DIFF_DISTRIB:
-  DISJOINT (A ∪ B DIFF C) D ⇔ DISJOINT (A DIFF C) D ∧ DISJOINT (B DIFF C) D
+Theorem perm1_list_unchanged:
+  ∀l x. ¬ MEM x (MAP FST l) ∧ ¬ MEM x (MAP SND l) ⇒ perm1_list l x = x
 Proof
-  fs[EXTENSION,DISJOINT_DEF,SUBSET_DEF] \\ metis_tac[]
+  recInduct perm1_list_ind >> rw[perm1_list_def] >>
+  gvs[perm1_def]
 QED
 
-Triviality DISJOINT_DIFF_WEAKENING:
-  DISJOINT A B ⇒ DISJOINT (A DIFF C) B
+Theorem perm1_list_fresh_var_list_correctness:
+  ∀l avoid A.
+    A ⊆ set avoid
+  ⇒ DISJOINT (IMAGE (perm1_list (fresh_var_list l avoid)) (set l)) A
 Proof
-  fs[EXTENSION,DISJOINT_DEF,SUBSET_DEF] \\ metis_tac[]
-QED
-
-Triviality FILTER_MAP_MEM:
-  ∀ l1 l2. MEM x l1 ∧ MEM x l2 ⇒ MEM x (nub (FILTER (λx. MEM x l1) l2))
-Proof
-  Induct_on ‘l1’ \\ fs[]
-  \\ rw[] \\ res_tac \\ fs[]
-  \\ Induct_on ‘l2’ \\ fs[]
-  \\ rw[] \\ res_tac \\ fs[]
-QED
-
-Triviality MEM_PAIR_MAP:
-  MEM (q,r) lcs ⇒ MEM q (MAP FST lcs)
-Proof
-  Induct_on ‘lcs’ \\ fs[]
-  \\ Cases \\ fs[] \\ rw[]
-  \\ res_tac \\ fs[]
-QED
-
-Triviality NOT_MEM_PAIR:
- (∀y. q ≠ FST y ∨ ¬MEM y l) ⇒ ¬MEM q (MAP FST l)
-Proof
-  Induct_on ‘l’ \\ fs[]
-  \\ Cases \\ fs[] \\ rw[]
-  THEN1 (
-    CCONTR_TAC \\ fs[] \\ rw[]
-    \\ last_x_assum mp_tac
-    \\ impl_tac THEN1 (metis_tac[MEM])
-    \\ fs[]
-    \\ pop_assum (qspec_then ‘(q,r)’ assume_tac) \\ fs[]
-  )
-  \\ last_x_assum irule
-  \\ rw[]
-  \\ pop_assum (qspec_then ‘y’ assume_tac) \\ fs[]
-QED
-
-Triviality NOT_MEM_DISJOINT:
-  ¬MEM x l ⇔ DISJOINT {x} (set l)
-Proof
-  fs[EXTENSION,DISJOINT_DEF] \\ metis_tac[MEM]
-QED
-
-Theorem avoid_vars_safe_renaming:
-  ∀ avoid e . freevars e ⊆ set avoid
-  ⇒ DISJOINT (boundvars (avoid_vars avoid e)) (set avoid)
-Proof
-  recInduct avoid_vars_ind
-  \\ rw[]
-  THEN1 (fs[avoid_vars_def])
-  THEN1 (
-    fs[avoid_vars_def]
-    \\ fs[MAP_MAP_o,combinTheory.o_DEF]
-    \\ fs[LIST_TO_SET_FLAT]
-    \\ fs[MAP_MAP_o,combinTheory.o_DEF]
-    \\ fs[MEM_MAP]
-    \\ fs[BIGUNION_SUBSET]
-    \\ rw[]
-    \\ last_x_assum irule
-    \\ fs[]
-    \\ first_x_assum (qspec_then ‘freevars a’ assume_tac)
-    \\ pop_assum irule
-    \\ fs[MEM_MAP]
-    \\ qexists_tac ‘a’ \\ fs[]
-  )
-  THEN1 (
-    ‘freevars e ⊆ x INSERT fresh_var x avoid INSERT set avoid’ by (
-      fs[EXTENSION,SUBSET_DEF] \\ metis_tac[]
-    )
-    \\ fs[] \\ pop_assum kall_tac
-    \\ fs[avoid_vars_def]
-    \\ rw[] \\ fs[fresh_var_correctness]
-    \\ simp[boundvars_perm_exp]
-    \\ rw[]
-    \\ fs[EXTENSION,DISJOINT_DEF,SUBSET_DEF] \\ metis_tac[fresh_var_correctness]
-  )
-  THEN1 (fs[avoid_vars_def])
-  \\ ‘freevars e ⊆
-        set (MAP FST lcs) ∪ set avoid ∪
-        set (MAP SND
-             (fresh_var_list (nub (FILTER (λx. MEM x avoid) (MAP FST lcs)))
-                (MAP FST lcs ++ avoid)))’ by (
-     fs[EXTENSION,SUBSET_DEF] \\ metis_tac[]
-  )
-  \\ fs[] \\ pop_assum kall_tac
-  \\ qspecl_then [‘(nub (FILTER (λx. MEM x avoid) (MAP FST lcs)))’
-                 ,‘(MAP FST lcs ++ avoid)’] assume_tac fresh_var_list_correctness
-  \\ fs[avoid_vars_def]
-  \\ fs[ZIP_MAP]
-  \\ fs[MAP_MAP_o,combinTheory.o_DEF]
-  \\ once_rewrite_tac[DISJOINT_SYM]
-  \\ irule DISJOINT_SUBSET
-  \\ qspecl_then
-     [‘(fresh_var_list
-                   (nub (FILTER (λx. MEM x avoid) (MAP FST lcs)))
-                   (MAP FST lcs ++ avoid))’
-     ,‘(Letrec
-                   (MAP
-                      (λx.
-                           (FST x,
-                            avoid_vars
-                              (MAP FST lcs ++ avoid ++
-                               MAP SND
-                                 (fresh_var_list
-                                    (nub
-                                       (FILTER (λx. MEM x avoid)
-                                          (MAP FST lcs)))
-                                    (MAP FST lcs ++ avoid))) (SND x))) lcs)
-                   (avoid_vars
-                      (MAP FST lcs ++ avoid ++
-                       MAP SND
-                         (fresh_var_list
-                            (nub (FILTER (λx. MEM x avoid) (MAP FST lcs)))
-                            (MAP FST lcs ++ avoid))) e))’]
-     mp_tac boundvars_perm_exp_list
-  \\ impl_tac
-  THEN1 (
-    fs[MAP_FST_fresh_var_list]
-    \\ conj_tac THEN1 (irule fresh_var_list_distinctness)
-    \\ conj_tac
-    THEN1 (fs[EXTENSION,DISJOINT_DEF,SUBSET_DEF] \\ metis_tac[])
-    \\ fs[MAP_MAP_o,combinTheory.o_DEF]
-    \\ fs[MEM_MAP]
-    \\ rw[]
-    \\ Cases_on ‘x’ \\ fs[]
-    \\ reverse conj_tac
-    THEN1 (
-      once_rewrite_tac[NOT_MEM_DISJOINT]
-      \\ once_rewrite_tac[DISJOINT_SYM]
-      \\ irule DISJOINT_SUBSET
-      \\ qexists_tac ‘set (MAP FST lcs ++ avoid)’
-      \\ fs[fresh_var_list_correctness]
-      \\ metis_tac[MEM_PAIR_MAP,MEM]
-    )
-    \\ res_tac \\ fs[]
-    \\ once_rewrite_tac[DISJOINT_SYM]
-    \\ first_assum irule
-    \\ irule SUBSET_TRANS
-    \\ qexists_tac ‘BIGUNION (set (MAP (λ(fn,e). freevars e) lcs))’
-    \\ reverse conj_tac THEN1 (fs[EXTENSION,SUBSET_DEF] \\ metis_tac[])
-    \\ irule SUBSET_BIGUNION_I
-    \\ fs[MEM_MAP]
-    \\ qexists_tac ‘(q,r)’ \\ fs[]
-  )
-  \\ strip_tac
-  \\ qexists_tac ‘ boundvars
-          (Letrec
-             (MAP
-                (λx.
-                     (FST x,
-                      avoid_vars
-                        (MAP FST lcs ++ avoid ++
-                         MAP SND
-                           (fresh_var_list
-                              (nub (FILTER (λx. MEM x avoid) (MAP FST lcs)))
-                              (MAP FST lcs ++ avoid))) (SND x))) lcs)
-             (avoid_vars
-                (MAP FST lcs ++ avoid ++
-                 MAP SND
-                   (fresh_var_list
-                      (nub (FILTER (λx. MEM x avoid) (MAP FST lcs)))
-                      (MAP FST lcs ++ avoid))) e)) DIFF
-        set
-          (MAP FST
-             (fresh_var_list (nub (FILTER (λx. MEM x avoid) (MAP FST lcs)))
-                (MAP FST lcs ++ avoid))) ∪
-        set
-          (MAP SND
-             (fresh_var_list (nub (FILTER (λx. MEM x avoid) (MAP FST lcs)))
-                (MAP FST lcs ++ avoid)))’
-  \\ fs[]
-  \\ reverse conj_tac THEN1 (
-    irule DISJOINT_SUBSET
-    \\ qexists_tac ‘set (MAP FST lcs ++ avoid)’
-    \\ fs[fresh_var_list_correctness]
-  )
-  \\ fs[DISJOINT_UNION_DIFF_DISTRIB]
-  \\ conj_tac THEN1 (fs[EXTENSION,DISJOINT_DEF,DIFF_DEF] \\ metis_tac[])
-  \\ fs[MAP_MAP_o,combinTheory.o_DEF]
-  \\ fs[pure_miscTheory.BIGUNION_DIFF]
-  \\ GEN_TAC
-  \\ rw[]
-  \\ fs[MEM_MAP]
-  \\ Cases_on ‘x’ \\ fs[] \\ rw[]
-  THEN1 (
-    res_tac \\ fs[]
-    \\ irule DISJOINT_DIFF_WEAKENING
-    \\ once_rewrite_tac[DISJOINT_SYM]
-    \\ first_assum irule
-    \\ irule SUBSET_TRANS
-    \\ qexists_tac ‘ BIGUNION (set (MAP (λ(fn,e). freevars e) lcs))’
-    \\ reverse conj_tac
-    THEN1 (fs[EXTENSION,DISJOINT_DEF,SUBSET_DEF] \\ metis_tac[])
-    \\ irule SUBSET_BIGUNION_I
-    \\ fs[MEM_MAP]
-    \\ qexists_tac ‘(FST y,r)’ \\ fs[]
-  )
-  THEN1 (
-    fs[MAP_FST_fresh_var_list]
-    \\ irule DISJOINT_DIFF_WEAKENING
-    \\ res_tac \\ fs[]
-    \\ once_rewrite_tac[DISJOINT_SYM]
-    \\ first_assum irule
-    \\ irule SUBSET_TRANS
-    \\ qexists_tac ‘BIGUNION (set (MAP (λ(fn,e). freevars e) lcs))’
-    \\ reverse conj_tac THEN1 (fs[EXTENSION,SUBSET_DEF] \\ metis_tac[])
-    \\ irule SUBSET_BIGUNION_I
-    \\ fs[MEM_MAP]
-    \\ qexists_tac ‘(q,r)’ \\ fs[]
-  )
-  \\ fs[]
-  \\ ‘¬MEM q (MAP FST (fresh_var_list (nub (FILTER (λx. MEM x avoid) (MAP FST lcs)))
-                      (MAP FST lcs ++ avoid)))’ by (
-     irule NOT_MEM_PAIR \\ fs[]
-  )
-  \\ CCONTR_TAC \\ fs[]
-  \\ ‘MEM q (nub (FILTER (λx. MEM x avoid) (MAP FST lcs)))’ by (
-    irule FILTER_MAP_MEM
-    \\ fs[]
-    \\ drule MEM_PAIR_MAP \\ fs[]
-  )
-  \\ ‘MEM q (MAP FST (fresh_var_list (nub (FILTER (λx. MEM x avoid) (MAP FST lcs)))
-                     (MAP FST lcs ++ avoid)))’ by (
-       qspecl_then [‘(nub (FILTER (λx. MEM x avoid) (MAP FST lcs)))’
-                   ,‘(MAP FST lcs ++ avoid)’] assume_tac MAP_FST_fresh_var_list
-       \\ metis_tac[MEM]
-     )
-  \\ fs[]
-QED
-
-Theorem boundvars_avoid_vars:
-∀l x. freevars body ⊆ set l ∧
-      MEM x (boundvars (avoid_vars l body)) ⇒
-        ¬MEM x l
-Proof
+  Induct >> rw[] >>
+  gvs[fresh_var_list_def, DISJOINT_DEF, EXTENSION,
+      DISJ_EQ_IMP, PULL_EXISTS, PULL_FORALL] >>
   rw[]
-  \\ qspecl_then [‘l’,‘body’] assume_tac avoid_vars_safe_renaming
-  \\ res_tac
-  \\ fs[EXTENSION,DISJOINT_DEF] \\ metis_tac[MEM]
+  >- (
+    simp[perm1_list_def] >>
+    qspecl_then [`h`,`avoid`] assume_tac fresh_var_DISJ >> gvs[perm1_simps]
+    >- (last_x_assum irule >> gvs[SUBSET_DEF]) >>
+    qabbrev_tac `fh = fresh_var h avoid` >> rename1 `MEM x l` >>
+    last_x_assum (qspecl_then [`fh::avoid`,`fh INSERT set avoid`] mp_tac) >>
+    simp[SUBSET_OF_INSERT] >> disch_then drule >> strip_tac >>
+    simp[perm1_def] >> gvs[SUBSET_DEF] >>
+    rw[] >> metis_tac[]
+    ) >>
+  qspecl_then [`h`,`avoid`] assume_tac fresh_var_DISJ >> gvs[]
+  >- (
+    simp[perm1_list_def, perm1_simps] >>
+    Cases_on `MEM h l`
+    >- (last_x_assum irule >> gvs[SUBSET_DEF]) >>
+    qsuff_tac `perm1_list (fresh_var_list l (h::avoid)) h = h`
+    >- (gvs[SUBSET_DEF] >> metis_tac[]) >>
+    irule perm1_list_unchanged >> simp[MAP_FST_fresh_var_list] >>
+    qspecl_then [`l`,`h::avoid`] assume_tac fresh_var_list_correctness >>
+    gvs[DISJOINT_DEF, EXTENSION] >> metis_tac[]
+    ) >>
+  qabbrev_tac `fh = fresh_var h avoid` >>
+  simp[perm1_list_def, perm1_def] >>
+  qspecl_then [`h`,`avoid`] assume_tac fresh_var_correctness >>
+  IF_CASES_TAC >- metis_tac[SUBSET_DEF] >>
+  qspecl_then [`l`,`fh::avoid`] assume_tac fresh_var_list_correctness >>
+  gvs[DISJOINT_DEF, EXTENSION] >>
+  pop_assum (qspec_then `h` assume_tac) >> gvs[] >>
+  Cases_on `¬MEM h l`
+  >- (drule_at Any perm1_list_unchanged >> simp[MAP_FST_fresh_var_list]) >>
+  gvs[] >> reverse IF_CASES_TAC
+  >- (last_x_assum irule >> gvs[SUBSET_DEF]) >>
+  last_x_assum (qspecl_then [`fh::avoid`,`fh INSERT set avoid`] assume_tac) >>
+  gvs[]
 QED
 
-Theorem subst_NOT_MEM:
- ∀ f arg.  ¬MEM n (freevars arg) ⇒ subst (f \\ n) arg = subst f arg
+Theorem freshen_safe_renaming:
+  ∀ avoid e.
+    freevars e ⊆ set avoid
+  ⇒ DISJOINT (boundvars (freshen avoid e)) (set avoid)
 Proof
-  recInduct subst_ind
-  \\ rw[]
-  THEN1 (fs[subst_def,DOMSUB_FLOOKUP_NEQ])
-  THEN1 (
-    fs[subst_def]
-    \\ fs[MAP_EQ_f]
-    \\ rw[] \\ res_tac \\ fs[]
-    \\ pop_assum irule
-    \\ fs[MEM_MAP] \\ metis_tac[MEM]
-  )
-  THEN1 (
-    fs[subst_def] \\ res_tac \\ fs[]
-  )
-  THEN1 (
-    fs[subst_def]
-    \\ fs[DOMSUB_COMMUTES]
-  )
-  THEN1 (
-    fs[subst_def]
-  )
-  THEN1 (
-    res_tac \\ fs[] \\ rw[]
-    \\ fs[subst_def]
-    \\ reverse conj_tac THEN1 (fs[fdiff_fdomsub_commute])
-    \\ fs[MEM_MAP]
-    \\ fs[MAP_EQ_f] \\ rw[]
-    \\ Cases_on ‘e’ \\ fs[]
-    \\ res_tac
-    \\ fs[fdiff_fdomsub_commute]
-    \\ pop_assum irule
-    \\ first_assum (qspec_then ‘freevars r’ assume_tac) \\ fs[]
-    \\ pop_assum (qspec_then ‘(q,r)’ assume_tac) \\ fs[]
-  )
-  \\ fs[subst_def]
-  \\ fs[fdiff_fdomsub_INSERT]
-  \\ ‘n INSERT set (MAP FST f) = set (MAP FST f)’ by (
-    fs[EXTENSION] \\ metis_tac[MEM]
-  )
-  \\ fs[]
+  recInduct freshen_ind >> rw[freshen_def]
+  >- (
+    gvs[DISJOINT_DEF, EXTENSION, DISJ_EQ_IMP] >> rw[] >>
+    gvs[MAP_MAP_o, combinTheory.o_DEF] >>
+    gvs[MEM_FLAT, MEM_MAP] >>
+    first_x_assum irule >> goal_assum drule >> simp[] >>
+    gvs[SUBSET_DEF] >> rw[] >>
+    last_x_assum irule >> simp[MEM_MAP, PULL_EXISTS] >>
+    goal_assum drule >> simp[]
+    )
+  >- (
+    gvs[DISJOINT_DEF, EXTENSION, DISJ_EQ_IMP] >> rw[] >>
+    gvs[IMP_CONJ_THM, FORALL_AND_THM] >>
+    first_x_assum irule >> gvs[GSYM SUBSET_INSERT_DELETE] >>
+    gvs[freevars_eqvt, SUBSET_DEF, PULL_EXISTS] >> rw[] >>
+    rename1 `z ∈ _` >> simp[perm1_def] >>
+    IF_CASES_TAC >> gvs[] >>
+    reverse IF_CASES_TAC >> gvs[] >- metis_tac[] >>
+    pop_assum mp_tac >> simp[Once fresh_var_def] >>
+    IF_CASES_TAC >> gvs[]
+    )
+  >- simp[fresh_var_correctness] >>
+  gvs[DIFF_SUBSET, AND_IMP_INTRO, GSYM CONJ_ASSOC] >>
+  qspecl_then [`MAP FST lcs`,`avoid`] assume_tac fresh_var_list_SUBSET >>
+  `freevars e ⊆
+    set (MAP SND (fresh_var_list (MAP FST lcs) avoid)) ∪ set avoid` by (
+      irule SUBSET_TRANS >> goal_assum drule >> simp[]) >>
+  gvs[] >> rw[boundvars_perm_exp_list]
+  >- (
+    qmatch_goalsub_abbrev_tac `IMAGE _ bvars` >>
+    `DISJOINT (set (MAP FST lcs)) bvars` by (
+      gvs[DISJOINT_DEF, EXTENSION, SUBSET_DEF] >> metis_tac[]) >>
+    gvs[DISJOINT_DEF, EXTENSION] >> rw[] >>
+    Cases_on `MEM x avoid` >> gvs[] >> rw[] >>
+    rename1 `_ ≠ _ z` >>
+    first_x_assum (qspec_then `z` assume_tac) >> gvs[] >>
+    first_x_assum (qspec_then `z` assume_tac) >> gvs[] >>
+    drule_at Any perm1_list_unchanged >> simp[MAP_FST_fresh_var_list] >>
+    strip_tac >>
+    Cases_on `x = z` >> gvs[] >> metis_tac[]
+    )
+  >- (
+    simp[MAP_MAP_o, combinTheory.o_DEF, LAMBDA_PROD] >>
+    simp[IMAGE_BIGUNION] >> rw[] >> pop_assum mp_tac >>
+    simp[MEM_MAP, PULL_EXISTS, FORALL_PROD] >> rw[] >>
+    qspecl_then [`MAP FST lcs`,`avoid`,`set avoid`]
+      assume_tac perm1_list_fresh_var_list_correctness >>
+    gvs[DISJOINT_DEF, EXTENSION, DISJ_EQ_IMP, PULL_EXISTS, MEM_MAP] >>
+    rw[] >> first_x_assum drule >> simp[GSYM FST_THM]
+    )
+  >- (
+    simp[MAP_MAP_o, combinTheory.o_DEF, LAMBDA_PROD] >>
+    simp[IMAGE_BIGUNION] >> rw[] >> pop_assum mp_tac >>
+    simp[MEM_MAP, PULL_EXISTS, FORALL_PROD] >> rw[] >>
+    qpat_x_assum `DISJOINT _ _` kall_tac >>
+    qpat_x_assum `DISJOINT _ _` kall_tac >>
+    ntac 2 $ qpat_x_assum `freevars e ⊆ _` kall_tac >>
+    last_x_assum drule >>
+    impl_tac
+    >- (
+      qpat_x_assum `BIGUNION _ ⊆ _` mp_tac >> simp[SUBSET_DEF, PULL_EXISTS] >>
+      simp[Once MEM_MAP, PULL_EXISTS, FORALL_PROD] >> rw[] >>
+      first_x_assum drule_all >> rw[] >> gvs[] >> gvs[SUBSET_DEF]
+      ) >>
+    strip_tac >>
+    gvs[DISJOINT_DEF, EXTENSION] >> rw[] >>
+    Cases_on `MEM x avoid` >> gvs[] >> rw[] >>
+    rename1 `z ∉ _` >>
+    first_assum (qspec_then `x` assume_tac) >>
+    first_x_assum (qspec_then `z` assume_tac) >> gvs[] >>
+    first_x_assum (qspec_then `z` assume_tac) >> gvs[] >>
+    gvs[SUBSET_DEF] >>
+    `¬ MEM z (MAP FST lcs)` by metis_tac[] >>
+    drule_at Any perm1_list_unchanged >> simp[MAP_FST_fresh_var_list] >>
+    strip_tac >> simp[DISJ_EQ_IMP] >> rw[] >> gvs[]
+    )
 QED
 
-Triviality MAP_FST_list_mono:
-  ∀ g l. MAP (λx. FST ((λ(f,e).(f,g e)) x)) l = MAP FST l
+Definition ca_subst_def:
+   ca_subst x arg body =
+       subst1 x arg (freshen (freevars_l arg ++ freevars_l body) body)
+End
+
+Theorem boundvars_freshen:
+  ∀avoid x body.
+    freevars body ⊆ set avoid ∧
+    MEM x (boundvars (freshen avoid body))
+    ⇒ ¬MEM x avoid
 Proof
-  rw[] \\ fs[MAP_EQ_f] \\ Cases \\ fs[]
+  rw[] >>
+  drule freshen_safe_renaming >> gvs[] >>
+  gvs[EXTENSION, DISJOINT_DEF] >>
+  metis_tac[]
 QED
 
-Triviality MAP_FST_MEM_pair_companion:
-  ∀x. MEM x (MAP FST lcs) ⇒ ∃ y. MEM (x,y) lcs
+Theorem FLOOKUP_FDIFF:
+  FLOOKUP (FDIFF fm s) k = if k ∈ s then NONE else FLOOKUP fm k
 Proof
-  rw[]
-  \\ Induct_on ‘lcs’ \\ fs[]
-  \\ Cases \\ fs[]
-  \\ Cases_on ‘x = q’ \\ fs[] \\ rw[]
-  \\ qexists_tac ‘r’ \\ fs[]
+  rw[FDIFF_def, FLOOKUP_DRESTRICT] >> gvs[]
 QED
 
-Triviality INSERT_absorption:
-  MEM x l ⇒ x INSERT (set l) = set l
+Theorem FDIFF_FUPDATE:
+  FDIFF (fm |+ (k,v)) s =
+  if k ∈ s then FDIFF fm s else (FDIFF fm s) |+ (k,v)
 Proof
-  fs[EXTENSION] \\ metis_tac[]
+  rw[fmap_eq_flookup, FLOOKUP_FDIFF, FLOOKUP_UPDATE] >>
+  EVERY_CASE_TAC >> gvs[]
 QED
 
-Theorem subst_distrib:
+Theorem FDIFF_FEMPTY[simp]:
+  FDIFF FEMPTY s = FEMPTY
+Proof
+  rw[fmap_eq_flookup, FLOOKUP_FDIFF]
+QED
+
+(* TODO prove more general version *)
+Theorem subst_single_distrib:
   ∀ body f v arg.
-    (∀n v. FLOOKUP f n = SOME v ⇒ closed v)
-  ∧ EVERY (λ x. x ∉ freevars arg) (boundvars body)
-   ⇒
-  subst f (subst v arg body)
-  = subst v (subst f arg) (subst (f \\ v) body)
+    (∀n v. FLOOKUP f n = SOME v ⇒ closed v) ∧
+    DISJOINT (freevars arg) (boundvars body)
+  ⇒ subst f (subst v arg body) = subst v (subst f arg) (subst (f \\ v) body)
 Proof
-  ho_match_mp_tac freevars_ind
-  \\ rpt strip_tac
-  THEN1(
-    fs[subst_def]
-    \\ fs[FLOOKUP_UPDATE] \\ fs[DOMSUB_FLOOKUP_THM]
-    \\ rw[] \\ fs[subst_single_def]
-    \\ Cases_on ‘FLOOKUP f n’ \\ fs[subst_single_def] \\ fs[subst_def]
-    \\ res_tac \\ fs[closed_subst])
-  THEN1(
-    fs[subst_def]
-    \\ fs[MAP_MAP_o,combinTheory.o_DEF]
-    \\ fs[MAP_EQ_f]
-    \\ fs[EVERY_FLAT,EVERY_MAP,EVERY_MEM]
-    \\ rw[] \\ res_tac \\ fs[]
-  )
-  THEN1(
-    fs[subst_def]
-    \\ res_tac \\ fs[]
-  )
-  THEN1(
-    fs[subst_single_def]
-    \\ IF_CASES_TAC \\ fs[subst_def]
-    \\ ‘∀m v. FLOOKUP (f \\ n) m = SOME v ⇒ closed v’ by (
-       fs[DOMSUB_FLOOKUP_THM]
-       \\ metis_tac[]
+  ho_match_mp_tac freevars_ind >> rw[]
+  >- (
+    gvs[subst_def, FLOOKUP_UPDATE, DOMSUB_FLOOKUP_THM] >>
+    EVERY_CASE_TAC >> gvs[subst_def, FLOOKUP_UPDATE] >>
+    last_x_assum drule >> simp[]
     )
-    \\ last_x_assum drule
-    \\ disch_then (qspecl_then [‘v’,‘arg’] mp_tac)
-    \\ impl_tac
-    \\ rw[]
-    \\ fs[DOMSUB_FUPDATE_NEQ]
-    \\ fs[subst_NOT_MEM]
-    \\ metis_tac[DOMSUB_COMMUTES]
-  )
-  \\ fs[MAP_MAP_o,combinTheory.o_DEF]
-  \\ fs[EVERY_FLAT,EVERY_MAP,EVERY_MEM]
-  \\ ‘∀ x. MEM x (MAP FST lcs) ⇒ ¬ MEM x (freevars arg)’ by (
-      rw[]
-      \\ last_assum irule
-      \\ imp_res_tac MAP_FST_MEM_pair_companion
-      \\ res_tac
-      \\ qexists_tac ‘(x,y)’ \\ fs[]
-  )
-  \\ fs[subst_def]
-  \\ fs[MAP_MAP_o,combinTheory.o_DEF]
-  \\ fs[MAP_FST_list_mono]
-  \\ fs[MAP_EQ_f]
-  \\ rw[]
-  \\ TRY (Cases_on ‘x’ \\ fs[])
-  \\ ‘(FDIFF (f \\ v) (set (MAP FST lcs))) = (FDIFF f (set (MAP FST lcs))) \\ v’ by (
-     simp[Once fdiff_fdomsub_commute]
-  ) \\ fs[] \\ pop_assum kall_tac
-  \\ ‘subst f arg = subst (FDIFF f (set (MAP FST lcs))) arg’ by (
-     irule subst_FDIFF'' \\ fs[]
-  ) \\ fs[] \\ pop_assum kall_tac
-  THEN1 (
-    last_x_assum (qspecl_then [‘q’,‘r’] mp_tac) \\ fs[]
-    \\ disch_tac
-    \\ simp[FDIFF_def]
-    \\ rw[]
-    \\ simp[GSYM FDIFF_def]
-    THEN1 (
-      first_assum irule
-      \\ rw[]
-      THEN1 (
-        first_assum irule
-        \\ qexists_tac ‘n’
-        \\ irule FLOOKUP_SUBMAP
-        \\ qexists_tac ‘(FDIFF f (set (MAP FST lcs)))’ \\ fs[]
-        \\ fs[FDIFF_def,DRESTRICT_SUBMAP]
-      )
-      \\ last_assum irule
-      \\ qexists_tac ‘(q,r)’ \\ fs[]
+  >- (
+    gvs[subst_def, MAP_MAP_o, combinTheory.o_DEF] >>
+    rw[MAP_EQ_f] >> last_x_assum irule >> simp[] >>
+    conj_tac >- metis_tac[] >>
+    gvs[MEM_MAP, PULL_EXISTS]
     )
-    \\ once_rewrite_tac[GSYM fdiff_fdomsub_commute]
-    \\ fs[fdiff_fdomsub_INSERT]
-    \\ fs[INSERT_absorption]
-  )
-  \\ simp[FDIFF_def]
-  \\ rw[]
-  \\ simp[GSYM FDIFF_def]
-  THEN1 (
-    first_assum irule
-    \\ rw[]
-    \\ first_assum irule
-    \\ qexists_tac ‘n’
-    \\ irule FLOOKUP_SUBMAP
-    \\ qexists_tac ‘(FDIFF f (set (MAP FST lcs)))’ \\ fs[]
-    \\ fs[FDIFF_def,DRESTRICT_SUBMAP]
-  )
-  \\ once_rewrite_tac[GSYM fdiff_fdomsub_commute]
-  \\ fs[fdiff_fdomsub_INSERT]
-  \\ fs[INSERT_absorption]
+  >- (
+    gvs[subst_def] >> rw[] >> first_x_assum irule >>
+    metis_tac[DISJOINT_SYM]
+    )
+  >- (
+    gvs[subst_single_def] >>
+    IF_CASES_TAC >> gvs[subst_def, DOMSUB_NOT_IN_DOM] >>
+    once_rewrite_tac[DOMSUB_COMMUTES] >>
+    `subst f arg = subst (f \\ n) arg` by (irule subst_fdomsub >> simp[]) >>
+    simp[] >>
+    last_x_assum irule >> simp[DOMSUB_FLOOKUP_THM] >> metis_tac[]
+    )
+  >- (
+    gvs[subst_def, MAP_MAP_o, combinTheory.o_DEF, LAMBDA_PROD] >>
+    gvs[GSYM FST_THM] >> rw[]
+    >- (
+      rw[MAP_EQ_f] >> pairarg_tac >> gvs[] >>
+      gvs[FDIFF_FUPDATE] >> IF_CASES_TAC >> gvs[]
+      >- (
+        gvs[fdiff_fdomsub_INSERT] >>
+        AP_THM_TAC >> rpt (AP_TERM_TAC) >>
+        rw[EXTENSION] >> eq_tac >> rw[] >> simp[]
+        ) >>
+      simp[fdiff_fdomsub_commute] >>
+      `subst f arg = subst (FDIFF f (set (MAP FST lcs))) arg` by (
+        irule subst_FDIFF'' >> rw[] >>
+        gvs[DISJOINT_DEF, EXTENSION, DISJ_EQ_IMP] >>
+        first_x_assum irule >>
+        gvs[MEM_MAP, PULL_EXISTS, EXISTS_PROD, FORALL_PROD] >>
+        goal_assum drule >> simp[]) >>
+      simp[] >>
+      last_x_assum irule >> simp[FLOOKUP_FDIFF] >> conj_tac >- metis_tac[] >>
+      simp[PULL_EXISTS] >> goal_assum (drule_at Any) >>
+      rw[Once DISJOINT_SYM] >>
+      qsuff_tac `DISJOINT (p1 INSERT boundvars p2) (freevars arg)` >- simp[] >>
+      first_x_assum irule >> gvs[MEM_MAP, EXISTS_PROD, FORALL_PROD] >>
+      goal_assum (drule_at Any) >> simp[]
+      ) >>
+    simp[FDIFF_FUPDATE] >> rw[]
+    >- (
+      simp[fdiff_fdomsub_INSERT] >> AP_THM_TAC >> rpt (AP_TERM_TAC) >>
+      rw[EXTENSION] >> eq_tac >> rw[] >> simp[]
+      ) >>
+    simp[fdiff_fdomsub_commute] >>
+    `subst f arg = subst (FDIFF f (set (MAP FST lcs))) arg` by (
+      irule subst_FDIFF'' >> rw[] >>
+      gvs[DISJOINT_DEF, EXTENSION, DISJ_EQ_IMP] >>
+      first_x_assum irule >>
+      gvs[MEM_MAP, PULL_EXISTS, EXISTS_PROD, FORALL_PROD] >>
+      goal_assum drule >> simp[]) >>
+    simp[] >>
+    first_x_assum irule >> simp[FLOOKUP_FDIFF] >> conj_tac >- metis_tac[] >>
+    simp[Once DISJOINT_SYM]
+    )
 QED
 
 Theorem beta_equivalence:
-  App (Lam x body) arg ≅ CA_subst x arg body
+  App (Lam x body) arg ≅ ca_subst x arg body
 Proof
-  fs[CA_subst_def]
-  \\ fs[exp_eq_def]
-  \\ rpt strip_tac
-  \\ fs[bind_def]
-  \\ rw[]
-  \\ fs[subst_def]
-  \\ match_mp_tac app_bisimilarity_trans
-  \\ qexists_tac ‘ subst x (subst f arg) (subst (f \\ x) body)’
-  \\ conj_tac
-  THEN1 (
-    irule App_Lam_bisim
-    \\ conj_tac THEN1 (
-      irule IMP_closed_subst \\ fs[FRANGE_DEF]
-      \\ fs[FLOOKUP_DEF,PULL_EXISTS]
-    )
-    \\ qsuff_tac ‘closed (subst f (Lam x body))’ THEN1 (fs[subst_def])
-    \\ irule IMP_closed_subst \\ fs[FRANGE_DEF]
-    \\ fs[FLOOKUP_DEF,PULL_EXISTS]
-  )
-  \\ drule subst_distrib
-  \\ disch_then (qspecl_then [‘(avoid_vars (freevars arg ++ freevars body) body)’
-                             ,‘x’,‘arg’] mp_tac)
-  \\ impl_tac
-  THEN1 (
-    fs[EVERY_MEM]
-    \\ rw[]
-    \\ imp_res_tac boundvars_avoid_vars \\ fs[]
-  )
-  \\ rw[]
-  \\ ‘(∀v. v ∈ FRANGE (f \\ x) ⇒ closed v)’ by (
-    rw[]
-    \\ first_assum irule
-    \\ fs[GSYM IN_FRANGE_FLOOKUP]
-    \\ fs[EXTENSION,FRANGE_DEF,IN_DEF] \\ rw[]
-    \\ fs[DOMSUB_FAPPLY_THM] \\ rw[]
-    \\ metis_tac[]
-  )
-  \\ fs[subst_subst_FUNION]
-  \\ irule app_bisimilarity_sym
-  \\ irule exp_alpha_app_bisimilarity
-  \\ reverse (rpt conj_tac)
-  THEN1 (
-    irule exp_alpha_subst_all_closed''
-    \\ rw[]
-    THEN1 (
-      qspecl_then [‘FEMPTY |+ (x,subst f arg)’,‘f \\ x’] mp_tac (GEN_ALL FRANGE_FUNION)
-      \\ impl_tac THEN1 (fs[FDOM_DOMSUB])
-      \\ disch_tac \\ fs[] \\ pop_assum kall_tac
-      \\ rw[]
-      \\ irule IMP_closed_subst \\ fs[]
-      \\ rw[]
-      \\ last_assum irule
-      \\ fs[GSYM IN_FRANGE_FLOOKUP]
-    )
-    \\ fs[exp_alpha_sym,exp_alpha_avoid_vars]
-  )
-  \\ irule IMP_closed_subst \\ fs[]
-  \\ rw[]
-  \\ TRY (
-    qspecl_then [‘FEMPTY |+ (x,subst f arg)’,‘f \\ x’] mp_tac (GEN_ALL FRANGE_FUNION)
-    \\ impl_tac THEN1 (fs[FDOM_DOMSUB])
-    \\ disch_tac \\ fs[] \\ pop_assum kall_tac
-    \\ rw[]
-    \\ irule IMP_closed_subst \\ fs[]
-    \\ rw[]
-    \\ last_assum irule
-    \\ fs[GSYM IN_FRANGE_FLOOKUP]
-  )
-  \\ fs[freevars_avoid_vars_mono]
-  \\ fs[EXTENSION,SUBSET_DEF] \\ metis_tac[]
+  fs[ca_subst_def, exp_eq_def] >> rw[bind_def, subst_def] >>
+  irule app_bisimilarity_trans >>
+  irule_at Any App_Lam_bisim >>
+  conj_asm1_tac
+  >- (
+    simp[] >> dep_rewrite.DEP_REWRITE_TAC[freevars_subst] >>
+    simp[IN_FRANGE_FLOOKUP, DOMSUB_FLOOKUP_THM] >> conj_tac >- metis_tac[] >>
+    gvs[SUBSET_DEF] >> metis_tac[]
+    ) >>
+  conj_asm1_tac
+  >- (
+    simp[closed_def] >> once_rewrite_tac[GSYM LIST_TO_SET_EQ_EMPTY] >>
+    dep_rewrite.DEP_REWRITE_TAC[freevars_subst] >> simp[IN_FRANGE_FLOOKUP] >>
+    simp[SUBSET_DIFF_EMPTY]
+    ) >>
+  dep_rewrite.DEP_REWRITE_TAC[subst1_distrib] >> rw[] >- metis_tac[]
+  >- (
+    qspecl_then [`freevars_l arg ++ freevars_l body`,`body`]
+      assume_tac freshen_safe_renaming >> gvs[] >>
+    gvs[freevars_equiv]
+    ) >>
+  dep_rewrite.DEP_REWRITE_TAC[subst_subst_FUNION] >>
+  simp[FUNION_FUPDATE_2, IN_FRANGE_FLOOKUP, DOMSUB_FLOOKUP_THM] >>
+  conj_tac >- (gvs[freevars_equiv] >> metis_tac[]) >>
+  irule exp_alpha_app_bisimilarity >>
+  simp[closed_def] >>
+  dep_rewrite.DEP_REWRITE_TAC[freevars_subst, freevars_freshen_mono] >>
+  simp[IN_FRANGE_FLOOKUP, FLOOKUP_UPDATE] >>
+  conj_asm1_tac
+  >- (rw[] >> EVERY_CASE_TAC >> gvs[freevars_equiv] >> metis_tac[]) >>
+  gvs[SUBSET_DIFF_EMPTY, SUBSET_INSERT_DELETE] >>
+  irule exp_alpha_subst_all_closed'' >>
+  simp[IN_FRANGE_FLOOKUP, FLOOKUP_UPDATE] >>
+  irule exp_alpha_freshen >> simp[]
 QED
 
 Theorem beta_bisimilarity:
   closed (Let x arg body) ⇒
-  Let x arg body ≃ CA_subst x arg body
+  Let x arg body ≃ ca_subst x arg body
 Proof
-  simp[app_bisimilarity_eq]
-  \\ rw[beta_equivalence]
-  \\ fs[CA_subst_def,closed_def]
-  \\ qspecl_then [‘x’,‘arg’,‘(avoid_vars (freevars body) body)’]
-                 assume_tac freevars_subst_single
-  \\ fs[closed_def] \\ res_tac \\ fs[]
-  \\ qsuff_tac ‘freevars (subst x arg (avoid_vars (freevars body) body)) = ∅’
-  THEN1 (fs[])
-  \\ pop_assum (fn t => once_rewrite_tac[t])
-  \\ qspecl_then [‘freevars body’,‘body’] mp_tac freevars_avoid_vars_mono
-  \\ fs[]
-  \\ rw[]
-  \\ fs[EXTENSION,SUBSET_DEF] \\ metis_tac[MEM]
+  rw[app_bisimilarity_eq, beta_equivalence] >>
+  simp[closed_def, ca_subst_def] >>
+  DEP_REWRITE_TAC [freevars_subst, freevars_freshen_mono] >>
+  simp[IN_FRANGE_FLOOKUP, FLOOKUP_UPDATE, SUBSET_DIFF_EMPTY] >>
+  gvs[freevars_equiv]
 QED
-
-
 
 (* TODO
 
